theories/Core/Soundness/EqualityCases.v
@@ -20,18 +20,14 @@ Lemma glu_rel_eq : forall Γ A i M N,
 Proof.
   intros * HA HM HN.
   assert {{ ⊩ Γ }} as [SbΓ] by mauto.
-  assert {{ Γ ⊢ A : Type@i }} by mauto.
-  assert {{ Γ ⊢ M : A }} by mauto.
-  assert {{ Γ ⊢ N : A }} by mauto.
-  invert_glu_rel_exp HA.
-  invert_glu_rel_exp HM.
-  invert_glu_rel_exp HN.
+  saturate_syn_judge.
+  invert_sem_judge.
 
   eapply glu_rel_exp_of_typ; mauto 3.
   intros.
   assert {{ Δ ⊢s σ : Γ }} by mauto 4.
   split; mauto 3.
-  applying_glu_rel_judge.
+  apply_glu_rel_judge.
   saturate_glu_typ_from_el.
   unify_glu_univ_lvl i.
   deepexec glu_univ_elem_per_univ ltac:(fun H => pose proof H).
@@ -49,7 +45,7 @@ Proof.
       assert {{ Δ' ⊢s τ : Δ }} by mauto 2;
       assert {{ Δ' ⊢s σ ∘ τ ® ρ ∈ SbΓ }} by (eapply glu_ctx_env_sub_monotone; eassumption);
       assert {{ Δ' ⊢s σ ∘ τ : Γ }} by mauto 2;
-      applying_glu_rel_judge;
+      apply_glu_rel_judge;
       handle_functional_glu_univ_elem;
       unify_glu_univ_lvl i.
     + bulky_rewrite.
@@ -68,13 +64,13 @@ Lemma glu_rel_eq_refl : forall Γ A M,
 Proof.
   intros * HM.
   assert {{ ⊩ Γ }} as [SbΓ] by mauto.
-  assert {{ Γ ⊢ M : A }} by mauto.
-  invert_glu_rel_exp HM.
+  saturate_syn_judge.
+  invert_sem_judge.
   assert {{ Γ ⊢ A : Type@x }} by mauto.
   eexists; split; eauto.
   exists x; intros.
   assert {{ Δ ⊢s σ : Γ }} by mauto 4.
-  applying_glu_rel_judge.
+  apply_glu_rel_judge.
   saturate_glu_typ_from_el.
   deepexec glu_univ_elem_per_univ ltac:(fun H => pose proof H).
   match_by_head per_univ ltac:(fun H => destruct H).
@@ -88,7 +84,7 @@ Proof.
     assert {{ Δ' ⊢s σ ∘ τ ® ρ ∈ SbΓ }} by (eapply glu_ctx_env_sub_monotone; eassumption);
     assert {{ Δ' ⊢s σ ∘ τ : Γ }} by mauto 2;
     assert {{ Δ' ⊢ M[σ][τ] ≈ M[σ ∘ τ] : A[σ ∘ τ] }} by mauto;
-    applying_glu_rel_judge;
+    apply_glu_rel_judge;
     saturate_glu_typ_from_el;
     bulky_rewrite.
 Qed.
